updated heapster example proofs to use prove_refinesFun

examples/heapster/linked_list_proofs.v
@@ -11,23 +11,26 @@ From CryptolToCoq Require Import CompMExtra.
 Load "linked_list.v".
 Import linked_list.
 
-Definition noErrorsSpec {A} : CompM A := existsM (fun a => returnM a).
-
 Import SAWCorePrelude.
 
 
 Lemma no_errors_is_elem : refinesFun is_elem (fun _ _ => noErrorsSpec).
 Proof.
-  unfold is_elem, is_elem__tuple_fun, noErrorsSpec.
-  apply refinesFun_multiFixM_fst. simpl. intros x l.
-  rewrite simpl_letRecM0.
-  apply refinesM_either; intros.
+  prove_refinesFun.
+Qed.
+
+Lemma no_errors_is_elem_manual : refinesFun is_elem (fun _ _ => noErrorsSpec).a
+Proof.
+  unfold noErrorsSpec.
+  apply refinesFun_multiFixM_fst. intros x l.
+  apply refinesM_letRecM0.
+  apply refinesM_either_l; intros.
   - eapply refinesM_existsM_r. reflexivity.
-  - apply refinesM_sigT_rect; intros.
-    apply refinesM_if; intros.
+  - apply refinesM_sigT_rect_l; intros.
+    apply refinesM_if_l; intros.
     + eapply refinesM_existsM_r. reflexivity.
     + rewrite existsM_bindM.
       apply refinesM_existsM_l; intros. rewrite returnM_bindM.
-      apply refinesM_sigT_rect; intros.
+      apply refinesM_sigT_rect_l; intros.
       eapply refinesM_existsM_r. reflexivity.
 Qed.
